jump_list_up_to

src/lowparse/LowParse.Low.ListUpTo.fst
@@ -134,3 +134,117 @@ let validate_list_up_to
   let res = B.index bpos 0ul in
   HST.pop_frame ();
   res
+
+unfold
+let jump_list_up_to_inv
+  (#k: _)
+  (#t: _)
+  (#p: parser k t)
+  (cond: (t -> Tot bool))
+  (prf: consumes_if_not_cond cond p { k.parser_kind_subkind <> Some ParserConsumesAll } )
+  (#rrel #rel: _)
+  (sl: slice rrel rel)
+  (pos0: U32.t)
+  (h0: HS.mem)
+  (bpos: B.pointer U32.t)
+  (h: HS.mem)
+  (stop: bool)
+: GTot Type0
+= let pos = B.deref h bpos in
+  let q = parse_list_up_to cond p prf in
+  B.live h0 bpos /\
+  live_slice h0 sl /\
+  B.loc_disjoint (B.loc_buffer sl.base) (B.loc_buffer bpos) /\
+  B.modifies (B.loc_buffer bpos) h0 h /\
+  U32.v pos0 <= U32.v pos /\
+  valid q h0 sl pos0 /\
+  begin if stop
+  then 
+    get_valid_pos q h0 sl pos0 == pos
+  else
+    valid q h0 sl pos /\
+    get_valid_pos q h0 sl pos0 == get_valid_pos q h0 sl pos
+  end
+
+#push-options "--z3rlimit 16"
+
+inline_for_extraction
+let jump_list_up_to_body
+  (#k: _)
+  (#t: _)
+  (#p: parser k t)
+  (cond: (t -> Tot bool))
+  (prf: consumes_if_not_cond cond p { k.parser_kind_subkind <> Some ParserConsumesAll } )
+  (j: jumper p)
+  (cond_impl: (
+    (#rrel: _) ->
+    (#rel: _) ->
+    (sl: slice rrel rel) ->
+    (pos: U32.t) ->
+    HST.Stack bool
+    (requires (fun h -> valid p h sl pos))
+    (ensures (fun h res h' ->
+      B.modifies B.loc_none h h' /\
+      valid p h sl pos /\
+      res == cond (contents p h sl pos)
+    ))
+  ))
+  (#rrel #rel: _)
+  (sl: slice rrel rel)
+  (pos0: U32.t)
+  (h0: HS.mem)
+  (bpos: B.pointer U32.t)
+: HST.Stack bool
+  (requires (fun h ->
+    jump_list_up_to_inv cond prf sl pos0 h0 bpos h false
+  ))
+  (ensures (fun h stop h' ->
+    jump_list_up_to_inv cond prf sl pos0 h0 bpos h false /\
+    jump_list_up_to_inv cond prf sl pos0 h0 bpos h' stop
+  ))
+=
+  let h = HST.get () in
+  let pos = B.index bpos 0ul in
+  valid_facts (parse_list_up_to cond p prf) h sl pos;
+  parse_list_up_to_eq cond p prf (bytes_of_slice_from h sl pos);
+  valid_facts p h sl pos;
+  let pos1 = j sl pos in
+  B.upd bpos 0ul pos1;
+  valid_facts (parse_list_up_to cond p prf) h sl pos1;
+  cond_impl sl pos
+
+#pop-options
+
+inline_for_extraction
+let jump_list_up_to
+  (#k: _)
+  (#t: _)
+  (#p: parser k t)
+  (cond: (t -> Tot bool))
+  (prf: consumes_if_not_cond cond p { k.parser_kind_subkind <> Some ParserConsumesAll } )
+  (j: jumper p)
+  (cond_impl: (
+    (#rrel: _) ->
+    (#rel: _) ->
+    (sl: slice rrel rel) ->
+    (pos: U32.t) ->
+    HST.Stack bool
+    (requires (fun h -> valid p h sl pos))
+    (ensures (fun h res h' ->
+      B.modifies B.loc_none h h' /\
+      valid p h sl pos /\
+      res == cond (contents p h sl pos)
+    ))
+  ))
+: Tot (jumper (parse_list_up_to cond p prf))
+= fun #rrel #rel sl pos ->
+  HST.push_frame ();
+  let bpos = B.alloca pos 1ul in
+  let h2 = HST.get () in
+  C.Loops.do_while
+    (jump_list_up_to_inv cond prf sl pos h2 bpos)
+    (fun _ -> jump_list_up_to_body cond prf j cond_impl sl pos h2 bpos)
+    ;
+  let res = B.index bpos 0ul in
+  HST.pop_frame ();
+  res
